src/dev/sttt/sttt_example.thy
@@ -1,20 +1,51 @@
 theory sttt_example
 imports sttt_setup
 begin
+section "the dist example"
+thm conj_disj_distribR ex_disj_distrib
+
+lemma "\<exists>x y. (x = y \<or> x > y) \<and> (x*x + y*y = (50::nat))"
+(*apply (subst conj_disj_distribR)
+apply (subst ex_disj_distrib)+*)
+apply (tinker disj)
+apply (rule disjI1)
+apply (rule_tac x = 5 in exI)+
+by simp
+
+
+
+
+section "the telephone example"
 typedecl Digitseq
 
 lemma running_example: "callee = Domain(call :: Digitseq rel) \<Longrightarrow> 
-       \<forall> x y. x \<in> callee \<and> y \<in> call `` {x} \<longrightarrow> x \<noteq> y \<Longrightarrow>
+       \<forall> x y. y \<in> call `` {x} \<longrightarrow> x \<noteq> y \<Longrightarrow>
        (s1 :: Digitseq) \<noteq> s2 \<Longrightarrow> 
-       \<exists> callee' call'. (\<forall> x y. x \<in> callee' \<and> y \<in> call' `` {x} \<longrightarrow> x \<noteq> y) \<and>
+       \<exists> callee' call'. (\<forall> x y. y \<in> call' `` {x} \<longrightarrow> x \<noteq> y) \<and>
          (callee' = Domain call') \<and> call' = call \<union> {(s1, s2)} "
-
+apply (tinker onep)
 ML_val {*- 
   val st =  Thm.cprem_of (#goal @{Isar.goal}) 1 |> Thm.term_of;
   val ps_thm = Tinker.start_ieval @{context} (SOME onep0) (SOME []) (SOME st) (* prove the goal *)
           |> EData.get_pplan |> IsaProver.get_goal_thm(* get the theorem *)
 *}
-oops
+
+apply (intro conjI) prefer 2 apply (rule refl) prefer 2 apply (rule refl) 
+find_theorems "(_ \<or> _)\<longrightarrow>_"
+thm Relation.Domain_Un_eq  Set.Un_iff Relation.Un_Image
+HOL.conj_disj_distribL HOL.conj_disj_distribR HOL.imp_disjL
+apply (subst Relation.Un_Image)
+apply (subst Set.Un_iff)+
+apply (subst HOL.imp_disjL)
+
+(* end of rippling, now pwf *)
+apply (intro allI) apply(erule_tac x = x in allE) apply(erule_tac x = y in allE)
+(* end of pwf forall *)
+apply (rule conjI)
+(*fertilisation*)
+apply (simp only:)
+(* auto *)
+apply simp
 ML{*-
   TextSocket.safe_close();
 *} 
